improve some proofs and progress in pack25519

Low/Get_abcdef.v
@@ -19,12 +19,22 @@ Definition get_f (t:(list Z * list Z * list Z * list Z * list Z * list Z)) : lis
   (a,b,c,d,e,f) => f
 end.
 
+Definition get_m (c:(list Z * list Z)) : list Z := match c with
+  (m,t) => m
+end.
+Definition get_t (c:(list Z * list Z)) : list Z := match c with
+  (m,t) => t
+end.
+
+
 Lemma get_a_length : forall a b c d e f, length (get_a (a,b,c,d,e,f)) = length a. Proof. go. Qed.
 Lemma get_b_length : forall a b c d e f, length (get_b (a,b,c,d,e,f)) = length b. Proof. go. Qed.
 Lemma get_c_length : forall a b c d e f, length (get_c (a,b,c,d,e,f)) = length c. Proof. go. Qed.
 Lemma get_d_length : forall a b c d e f, length (get_d (a,b,c,d,e,f)) = length d. Proof. go. Qed.
 Lemma get_e_length : forall a b c d e f, length (get_e (a,b,c,d,e,f)) = length e. Proof. go. Qed.
 Lemma get_f_length : forall a b c d e f, length (get_f (a,b,c,d,e,f)) = length f. Proof. go. Qed.
+Lemma get_m_length : forall m t, length (get_m (m,t)) = length m. Proof. go. Qed.
+Lemma get_t_length : forall m t, length (get_t (m,t)) = length t. Proof. go. Qed.
 
 Open Scope Z.
 
@@ -34,5 +44,7 @@ Lemma get_c_Zlength : forall a b c d e f, Zlength (get_c (a,b,c,d,e,f)) = Zlengt
 Lemma get_d_Zlength : forall a b c d e f, Zlength (get_d (a,b,c,d,e,f)) = Zlength d. Proof. go. Qed.
 Lemma get_e_Zlength : forall a b c d e f, Zlength (get_e (a,b,c,d,e,f)) = Zlength e. Proof. go. Qed.
 Lemma get_f_Zlength : forall a b c d e f, Zlength (get_f (a,b,c,d,e,f)) = Zlength f. Proof. go. Qed.
+Lemma get_m_Zlength : forall m t, Zlength (get_m (m,t)) = Zlength m. Proof. go. Qed.
+Lemma get_t_Zlength : forall m t, Zlength (get_t (m,t)) = Zlength t. Proof. go. Qed.
 
 Close Scope Z.
