Low/Reduce_by_P.v
@@ -1,6 +1,7 @@
 From Tweetnacl Require Import Libs.Export.
 From Tweetnacl Require Import ListsOp.Export.
 From Tweetnacl Require Import Mid.SubList.
+From Tweetnacl Require Import Low.Get_abcdef.
 From stdpp Require Import prelude.
 Require Import Recdef.
 
@@ -40,53 +41,128 @@ Open Scope Z.
 0x7fff = 32767
 *)
 
+Section val_sec.
+
 Definition subst_0xffed t := t - 65517.
 Definition subst_0xffff t m := t - 65535 - (Z.land (Z.shiftr m 16) 1).
 Definition subst_0x7fff t m := t - 32767 - (Z.land (Z.shiftr m 16) 1).
 Definition mod0xffff m := Z.land m 65535.
 Definition getBit256 l := Z.land (Z.shiftr (nth 15%nat l 0) 16) 1.
 
-Definition step_sub (a:Z) (m t:list Z) : list Z :=
+Definition sub_step (a:Z) (m t:list Z) : list Z :=
     let m' := nth (Z.to_nat (a - 1)) m 0 in
     let t' := nth (Z.to_nat a) t 0 in
       upd_nth (Z.to_nat (a-1)) (upd_nth (Z.to_nat a) m (subst_0xffff t' m')) (mod0xffff m').
 
-Function sub_fn_rev (a:Z) (m t: list Z) {measure Z.to_nat a} : (list Z) :=
-  if (a <=? 0)
+(* Definition of the for loop : 1 -> 15 *)
+Function sub_fn_rev (f:Z -> list Z -> list Z -> list Z) (a:Z) (m t: list Z) {measure Z.to_nat a} : (list Z) :=
+  if (a <=? 1)
     then m
     else
-      let prev := sub_fn_rev (a - 1) m t in 
-        step_sub a prev t.
+      let prev := sub_fn_rev f (a - 1) m t in 
+        f (a - 1) prev t.
 Proof. intros. apply Z2Nat.inj_lt ; move: teq ; rewrite Z.leb_gt => teq; omega. Defined.
 
-Lemma sub_fn_rev_0 : forall m t,
-  sub_fn_rev 0 m t = m.
+Lemma sub_fn_rev_1 : forall f m t,
+  sub_fn_rev f 1 m t = m.
 Proof. go. Qed.
 
-Lemma sub_fn_rev_n : forall a m t,
-  0 < a ->
-  sub_fn_rev a m t = step_sub a (sub_fn_rev (a - 1) m t) t.
+Lemma sub_fn_rev_n : forall a m t f,
+  1 < a ->
+  sub_fn_rev f a m t = f (a - 1) (sub_fn_rev f (a - 1) m t) t.
 Proof. intros. rewrite sub_fn_rev_equation.
 flatten ; apply Zle_bool_imp_le in Eq; omega.
 Qed.
 
 Definition m_from_t (m t:list Z) : list Z := 
   let m0 := upd_nth 0 m (subst_0xffed (nth 0 t 0)) in
-  let m14 := sub_fn_rev 14 m0 t in
+  let m14 := sub_fn_rev sub_step 15 m0 t in
   let m15 := upd_nth 15 m14 (subst_0x7fff (nth 15 t 0) (nth 14 m14 0)) in
   upd_nth 14 m15 (mod0xffff (nth 14 m15 0)).
 
-(*
-Definition list25519 := [65517;65535;65535;65535;65535;65535;65535;65535;65535;65535;65535;65535;65535;65535;65535;32767].
-Lemma list_of_P: forall l,
-  l = list25519 ->
-  (ZofList 16 l) = Z.pow 2 255 - 19.
-Proof. intros; subst; compute ; reflexivity. Qed.
-*)
+Lemma subst_select_step_Zlength : forall i m t,
+  0 < i < 16->
+  Zlength m = 16 ->
+  Zlength (sub_step i m t) = 16.
+Proof.
+  intros.
+  rewrite /sub_step.
+  assert(0 < Z.to_nat i /\ Z.to_nat i < 16) by (rewrite ?Z2Nat.id ; omega).
+  assert(Z.of_nat (Z.to_nat (i - 1)) = (Z.of_nat (Z.to_nat i)) - 1) by (rewrite ?Z2Nat.id ; omega).
+  rewrite ?upd_nth_Zlength ; omega.
+Qed.
+
+Lemma sub_fn_rev_Zlength_ind_step : forall i m t,
+  0 < i < 16 ->
+  Zlength m = 16 ->
+  Zlength (sub_fn_rev sub_step i m t) = 16 ->
+  Zlength (sub_fn_rev sub_step (i+1) m t) = 16.
+Proof.
+intros.
+rewrite sub_fn_rev_equation.
+flatten.
+replace ( i + 1 - 1) with i by omega.
+apply subst_select_step_Zlength=> //.
+Qed.
+
+Lemma sub_fn_rev_val_Zlength : forall i m t,
+  0 < i < 16 -> 
+  Zlength m = 16 ->
+  Zlength (sub_fn_rev sub_step i m t) = 16.
+Proof.
+intros.
+change(Zlength (sub_fn_rev sub_step i m t) = 16) with
+  ((fun x => Zlength (sub_fn_rev sub_step x m t) = 16) i).
+apply P016_impl.
+by rewrite sub_fn_rev_1.
+intros ; by apply sub_fn_rev_Zlength_ind_step.
+trivial.
+Qed.
 
 
 
 
 
+
+
+
+
+
+
+
+
+
+
+
+
+
+
+
+
+Function subst_select (f:Z -> list Z -> list Z -> list Z*list Z) (a:Z) (m t: list Z) {measure Z.to_nat a} : (list Z*list Z) :=
+  if (a <=? 0)
+    then (m,t)
+    else
+      let m_prev := get_m (subst_select f (a - 1) m t) in 
+      let t_prev := get_t (subst_select f (a - 1) m t) in 
+        (f a m_prev t_prev).
+Proof. intros. apply Z2Nat.inj_lt ; move: teq ; rewrite Z.leb_gt => teq; omega. Defined.
+
+Lemma subst_select_0 : forall f m t,
+  subst_select f 0 m t = (m,t).
+Proof. go. Qed.
+
+Lemma subst_select_n : forall a m t f,
+  0 < a ->
+  subst_select f a m t = (f a (get_m (subst_select f (a - 1) m t)) (get_t (subst_select f (a - 1) m t))).
+Proof. intros. rewrite subst_select_equation.
+flatten ; apply Zle_bool_imp_le in Eq; omega.
+Qed.
+
+
+
+
+
+End val_sec.
 
 Close Scope Z.
